Port more of the old code into the streaming functor. Rewrite several proofs without nonlinear arithmetic. Flesh out several other proofs for reliable verification.

code/streaming/Hacl.Streaming.Functor.fst
@@ -6,7 +6,7 @@ module Hacl.Streaming.Functor
 /// of the index, and a type class for that index. Then, as usual, a given value
 /// for the index as a parameter.
 
-#set-options "--max_fuel 0 --max_ifuel 0 --z3rlimit 100"
+#set-options "--max_fuel 0 --max_ifuel 0"
 
 module ST = FStar.HyperStack.ST
 module HS = FStar.HyperStack
@@ -28,6 +28,7 @@ inline_for_extraction noextract
 let uint32 = Lib.IntTypes.uint32
 
 /// State machinery
+/// ===============
 
 noeq
 type state_s #index (c: block index) (i: index) =
@@ -59,27 +60,28 @@ let footprint #index (c: block index) (i: index) (m: HS.mem) (s: state c i) =
   B.(loc_union (loc_addr_of_buffer s) (footprint_s c i m (B.deref m s)))
 
 /// Invariants
+/// ==========
 
 noextract
 let bytes = S.seq uint8
 
 noextract
-let split_at_last (block_length: pos) (b: bytes):
+let split_at_last #index (c: block index) (i: index) (b: bytes):
   Pure (bytes & bytes)
     (requires True)
     (ensures (fun (blocks, rest) ->
-      S.length rest < block_length /\
-      S.length rest = S.length b % block_length /\
+      S.length rest < U32.v (c.block_len i) /\
+      S.length rest = S.length b % U32.v (c.block_len i) /\
       S.equal (S.append blocks rest) b /\
-      S.length blocks % block_length = 0))
+      S.length blocks % U32.v (c.block_len i) = 0))
 =
-  let n = S.length b / block_length in
-  let blocks, rest = S.split b (n * block_length) in
-  assert (S.length blocks = n * block_length);
-  FStar.Math.Lemmas.multiple_modulo_lemma n block_length;
-  assert ((n * block_length) % block_length = 0);
-  assert (S.length rest = S.length b - n * block_length);
-  assert (S.length b - n * block_length < block_length);
+  let n = S.length b / U32.v (c.block_len i) in
+  let blocks, rest = S.split b (n * U32.v (c.block_len i)) in
+  assert (S.length blocks = n * U32.v (c.block_len i));
+  FStar.Math.Lemmas.multiple_modulo_lemma n (U32.v (c.block_len i));
+  assert ((n * U32.v (c.block_len i)) % U32.v (c.block_len i) = 0);
+  assert (S.length rest = S.length b - n * U32.v (c.block_len i));
+  assert (S.length b - n * U32.v (c.block_len i) < U32.v (c.block_len i));
   blocks, rest
 
 let loc_includes_union_l_footprint_s
@@ -99,7 +101,7 @@ let loc_includes_union_l_footprint_s
 let invariant_s #index (c: block index) (i: index) h (s: state_s c i) =
   let State hash_state buf_ total_len seen = s in
   let seen = G.reveal seen in
-  let blocks, rest = split_at_last (U32.v (c.block_len i)) seen in
+  let blocks, rest = split_at_last c i seen in
 
   // Liveness and disjointness (administrative)
   B.live h buf_ /\ c.invariant #i h hash_state /\
@@ -197,9 +199,9 @@ val create_in (#index: Type0) (c: block index) (i: index) (r: HS.rid): ST (state
     B.(loc_includes (loc_region_only true r) (footprint c i h1 s)) /\
     freeable c i h1 s))
 
-let split_at_last_empty (block_length: pos): Lemma
+let split_at_last_empty #index (c: block index) (i: index): Lemma
   (ensures (
-    let blocks, rest = split_at_last block_length S.empty in
+    let blocks, rest = split_at_last c i S.empty in
     S.equal blocks S.empty /\ S.equal rest S.empty))
 =
   ()
@@ -244,7 +246,7 @@ let create_in #index c i r =
   (**) assert (B.fresh_loc (c.footprint #i h4 hash_state) h0 h4);
   (**) assert (B.fresh_loc (B.loc_buffer buf) h0 h4);
   (**) c.update_multi_zero i (c.v h4 hash_state);
-  (**) split_at_last_empty (U32.v (c.block_len i));
+  (**) split_at_last_empty c i;
   (**) B.modifies_only_not_unused_in B.loc_none h0 h4;
 
   (**) let h5 = ST.get () in
@@ -253,7 +255,7 @@ let create_in #index c i r =
     let s = (B.get h5 p 0) in
     let State hash_state buf_ total_len seen = s in
     let seen = G.reveal seen in
-    let blocks, rest = split_at_last (U32.v (c.block_len i)) seen in
+    let blocks, rest = split_at_last c i seen in
     // JP: unclear why I need to assert this... but without it the proof doesn't
     // go through.
     U64.v total_len < c.max_input_length i /\
@@ -318,7 +320,7 @@ let init #index c i s =
   c.init (G.hide i) hash_state;
   let h2 = ST.get () in
   c.update_multi_zero i (c.v h2 hash_state);
-  split_at_last_empty U32.(v (c.block_len i));
+  split_at_last_empty c i;
 
   B.upd s 0ul (State hash_state buf 0UL (G.hide S.empty));
   let h3 = ST.get () in
@@ -341,7 +343,7 @@ let init #index c i s =
     let s = B.get h3 s 0 in
     let State hash_state buf_ total_len seen = s in
     let seen = G.reveal seen in
-    let blocks, rest = split_at_last (U32.v (c.block_len i)) seen in
+    let blocks, rest = split_at_last c i seen in
 
     // Liveness and disjointness (administrative)
     B.live h buf_ /\ c.invariant #i h hash_state /\
@@ -394,13 +396,45 @@ let update_post
 /// this stage in having an agile type for lengths that would be up to 2^125 for
 /// SHA384/512.
 
+#push-options "--z3cliopt smt.arith.nl=false"
+let mod_block_len_bound #index (c: block index) (i: index)
+  (total_len: U64.t): Lemma
+  (requires True)
+  (ensures U64.v (total_len `U64.rem` FStar.Int.Cast.uint32_to_uint64 (c.block_len i)) <= pow2 32 - 1)
+=
+  let open FStar.Int.Cast in
+  let x = total_len `U64.rem` uint32_to_uint64 (c.block_len i) in
+  calc (<=) {
+    U64.v x;
+  (<=) { FStar.Math.Lemmas.euclidean_division_definition (U64.v total_len) (U64.v (uint32_to_uint64 (c.block_len i))) }
+    U64.v total_len % U64.v (uint32_to_uint64 (c.block_len i) );
+  (<=) { FStar.Math.Lemmas.modulo_range_lemma (U64.v total_len) (U64.v (uint32_to_uint64 (c.block_len i))) }
+    U64.v (uint32_to_uint64 (c.block_len i));
+  (<=) { }
+    pow2 32 - 1;
+  }
+
 inline_for_extraction noextract
 let rest #index (c: block index) (i: index)
   (total_len: UInt64.t): (x:UInt32.t { U32.v x = U64.v total_len % U32.v (c.block_len i) })
 =
   let open FStar.Int.Cast in
-  assert (uint32_to_uint64 (c.block_len i) <> 0UL);
-  uint64_to_uint32 (total_len `U64.rem` uint32_to_uint64 (c.block_len i))
+  let x = total_len `U64.rem` uint32_to_uint64 (c.block_len i) in
+  let r = FStar.Int.Cast.uint64_to_uint32 x in
+  mod_block_len_bound c i total_len;
+  calc (==) {
+    U32.v r;
+  (==) { }
+    U64.v x % pow2 32;
+  (==) { FStar.Math.Lemmas.small_modulo_lemma_1 (U64.v x) (pow2 32) }
+    U64.v x;
+  (==) { FStar.Math.Lemmas.euclidean_division_definition (U64.v total_len) (U64.v (uint32_to_uint64 (c.block_len i))) }
+    U64.v total_len % U64.v (uint32_to_uint64 (c.block_len i) );
+  (==) { }
+    U64.v total_len % U32.v (c.block_len i);
+  };
+  r
+#pop-options
 
 inline_for_extraction noextract
 let add_len #index (c: block index) (i: index) (total_len: UInt64.t) (len: UInt32.t):
@@ -409,3 +443,522 @@ let add_len #index (c: block index) (i: index) (total_len: UInt64.t) (len: UInt3
     (ensures fun x -> U64.v x = U64.v total_len + U32.v len /\ U64.v x < c.max_input_length i)
 =
   total_len `U64.add` Int.Cast.uint32_to_uint64 len
+
+/// We split update into several versions, to all be simplified into a single
+/// large one at extraction-time.
+
+let total_len_h #index (c: block index) (i: index) h (p: state c i) =
+  State?.total_len (B.deref h p)
+
+/// Case 1: we just need to grow the buffer, no call to the hash function.
+
+#push-options "--z3rlimit 50"
+let split_at_last_small #index (c: block index) (i: index) (b: bytes) (d: bytes): Lemma
+  (requires (
+    let _, rest = split_at_last c i b in
+    S.length rest + S.length d < U32.v (c.block_len i)))
+  (ensures (
+    let blocks, rest = split_at_last c i b in
+    let blocks', rest' = split_at_last c i (S.append b d) in
+    S.equal blocks blocks' /\ S.equal (S.append rest d) rest'))
+=
+  let blocks, rest = split_at_last c i b in
+  let blocks', rest' = split_at_last c i (S.append b d) in
+  let l = U32.v (c.block_len i) in
+
+  (* Looking at the definition of split_at_last, blocks depends only on S.length b / l. *)
+  calc (==) {
+    S.length b / l;
+  (==) { S.lemma_len_append blocks rest }
+    (S.length blocks + S.length rest) / l;
+  (==) { Math.Lemmas.lemma_div_exact (S.length blocks) l }
+    (l * (S.length blocks / l) + S.length rest) / l;
+  (==) { }
+    (S.length rest + (S.length blocks / l) * l) / l;
+  (==) { Math.Lemmas.lemma_div_plus (S.length rest) (S.length blocks / l) l }
+    (S.length rest) / l + (S.length blocks / l);
+  (==) { Math.Lemmas.small_div (S.length rest) l }
+    S.length blocks / l;
+  };
+
+  calc (==) {
+    S.length (S.append b d) / l;
+  (==) { S.lemma_len_append b d; S.lemma_len_append blocks rest }
+    (S.length blocks + S.length rest + S.length d) / l;
+  (==) { Math.Lemmas.lemma_div_exact (S.length blocks) l }
+    (l * (S.length blocks / l) + (S.length rest + S.length d)) / l;
+  (==) { }
+    ((S.length rest + S.length d) + (S.length blocks / l) * l) / l;
+  (==) { Math.Lemmas.lemma_div_plus (S.length rest + S.length d) (S.length blocks / l) l }
+    (S.length rest + S.length d) / l + (S.length blocks / l);
+  (==) { Math.Lemmas.small_div (S.length rest + S.length d) l }
+    S.length blocks / l;
+  };
+
+  assert (S.equal blocks blocks');
+
+  calc (S.equal) {
+    rest `S.append` d;
+  (S.equal) { (* definition *) }
+    S.slice b ((S.length b / l) * l) (S.length b) `S.append` d;
+  (S.equal) { }
+    S.slice (S.append b d) ((S.length b / l) * l) (S.length b) `S.append` d;
+  (S.equal) { (* above *) }
+    S.slice (S.append b d) ((S.length (S.append b d) / l) * l) (S.length b) `S.append` d;
+  (S.equal) { (* ? *) }
+    S.slice (S.append b d) ((S.length (S.append b d) / l) * l) (S.length b)
+    `S.append`
+    S.slice (S.append b d) (S.length b) (S.length (S.append b d));
+  (S.equal) { S.lemma_split (S.append b d) ((S.length (S.append b d) / l) * l) }
+    S.slice (S.append b d) ((S.length (S.append b d) / l) * l) (S.length b + S.length d);
+  (S.equal) { S.lemma_len_append b d }
+    S.slice (S.append b d) ((S.length (S.append b d) / l) * l) (S.length (S.append b d));
+  (S.equal) { }
+    rest';
+  };
+
+  ()
+#pop-options
+
+#push-options "--z3cliopt smt.arith.nl=false"
+let add_len_small #index (c: block index) (i: index) (total_len: UInt64.t) (len: UInt32.t): Lemma
+  (requires
+    U32.v len < U32.v (c.block_len i) - U32.v (rest c i total_len) /\
+    U64.v total_len + U32.v len < c.max_input_length i)
+  (ensures (rest c i (add_len c i total_len len) = rest c i total_len `U32.add` len))
+=
+  calc (==) {
+    U32.v (rest c i (add_len c i total_len len));
+  (==) { }
+    U64.v (add_len c i total_len len) % U32.v (c.block_len i);
+  (==) { }
+    (U64.v total_len + U32.v len) % U32.v (c.block_len i);
+  (==) { Math.Lemmas.modulo_distributivity (U64.v total_len) (U32.v len) (U32.v (c.block_len i)) }
+    (U64.v total_len % U32.v (c.block_len i) + U32.v len % U32.v (c.block_len i)) % U32.v (c.block_len i);
+  (==) { Math.Lemmas.lemma_mod_add_distr (U64.v total_len % U32.v (c.block_len i)) (U32.v len) (U32.v (c.block_len i)) }
+    (U64.v total_len % U32.v (c.block_len i) + U32.v len) % U32.v (c.block_len i);
+  (==) { }
+    (U32.v (rest c i total_len) + U32.v len) % U32.v (c.block_len i);
+  (==) { Math.Lemmas.modulo_lemma (U32.v (rest c i total_len) + U32.v len) (U32.v (c.block_len i)) }
+    U32.v (rest c i total_len) + U32.v len;
+  }
+#pop-options
+
+val update_small:
+  #index:Type0 ->
+  (c: block index) ->
+  i:G.erased index -> (
+  let i = G.reveal i in
+  s:state c i ->
+  data: B.buffer uint8 ->
+  len: UInt32.t ->
+  Stack unit
+    (requires fun h0 ->
+      update_pre c i s data len h0 /\
+      U32.v len < U32.v (c.block_len i) - U32.v (rest c i (total_len_h c i h0 s)))
+    (ensures fun h0 s' h1 ->
+      update_post c i s data len h0 h1))
+
+#push-options "--z3rlimit 50"
+let update_small #index c i p data len =
+  let aux (h:HS.mem) (s:c.state i): Lemma
+    (requires (c.invariant h s))
+    (ensures (B.loc_in (c.footprint #i h s) h))
+    [SMTPat (c.invariant h s)]
+  =
+    c.invariant_loc_in_footprint #i h s
+  in
+  let aux l s h0 h1: Lemma
+    (requires
+      c.invariant h0 s /\
+      c.freeable h0 s /\
+      B.loc_disjoint l (c.footprint #i h0 s) /\
+      B.modifies l h0 h1)
+    (ensures (
+      c.freeable h1 s))
+    [ SMTPat (c.freeable h1 s); SMTPat (B.modifies l h0 h1) ]
+  =
+    c.frame_freeable #i l s h0 h1
+  in
+  let open LowStar.BufferOps in
+  let h00 = ST.get () in
+  assert (invariant c i h00 p);
+  let s = !*p in
+  let State hash_state buf total_len seen_ = s in
+  let i = c.index_of_state i hash_state in
+  [@inline_let]
+  let hash_state: c.state i = hash_state in
+
+  let sz = rest c i total_len in
+  add_len_small c i total_len len;
+  let h0 = ST.get () in
+  let buf1 = B.sub buf 0ul sz in
+  let buf2 = B.sub buf sz len in
+
+  B.blit data 0ul buf2 0ul len;
+  let h1 = ST.get () in
+  split_at_last_small c i (G.reveal seen_) (B.as_seq h0 data);
+  c.frame_invariant (B.loc_buffer buf) hash_state h0 h1;
+  assert (B.as_seq h1 data == B.as_seq h0 data);
+
+  let total_len = add_len c i total_len len in
+  p *= (State hash_state buf total_len (G.hide (G.reveal seen_ `S.append` (B.as_seq h0 data))));
+  let h2 = ST.get () in
+  assert (B.as_seq h2 data == B.as_seq h1 data);
+  c.frame_invariant (B.loc_buffer p) hash_state h1 h2;
+  assert (
+    let b = S.append (G.reveal seen_) (B.as_seq h0 data) in
+    let blocks, rest = split_at_last c i b in
+    S.length blocks + S.length rest = U64.v total_len /\
+    S.length b = U64.v total_len /\
+    U64.v total_len < c.max_input_length i /\
+    (==) (c.v h2 hash_state) (c.update_multi_s i (c.init_s i) blocks) /\
+    S.equal (S.slice (B.as_seq h2 buf) 0 (U64.v total_len % U32.v (c.block_len i))) rest
+    );
+  assert (seen c i h2 p `S.equal` (S.append (G.reveal seen_) (B.as_seq h0 data)));
+  assert (footprint c i h0 p == footprint c i h2 p);
+  assert (preserves_freeable c i p h0 h2);
+  assert (equal_domains h00 h2)
+
+#pop-options
+
+/// Case 2: we have no buffered data.
+
+#set-options "--z3rlimit 60"
+let split_at_last_blocks #index (c: block index) (i: index) (b: bytes) (d: bytes): Lemma
+  (requires (
+    let blocks, rest = split_at_last c i b in
+    S.equal rest S.empty))
+  (ensures (
+    let blocks, rest = split_at_last c i b in
+    let blocks', rest' = split_at_last c i d in
+    let blocks'', rest'' = split_at_last c i (S.append b d) in
+    S.equal blocks'' (S.append blocks blocks') /\
+    S.equal rest' rest''))
+=
+  let blocks, rest = split_at_last c i b in
+  let blocks', rest' = split_at_last c i d in
+  let blocks'', rest'' = split_at_last c i (S.append b d) in
+  let b' = S.append blocks rest in
+  let d' = S.append blocks' rest' in
+  let l = U32.v (c.block_len i) in
+  calc (S.equal) {
+    rest';
+  (S.equal) { }
+    snd (split_at_last c i d);
+  (S.equal) { }
+    S.slice d ((S.length d / l) * l) (S.length d);
+  (S.equal) { }
+    S.slice (S.append b d) (S.length b + (S.length d / l) * l) (S.length b + S.length d);
+  (S.equal) { }
+    S.slice (S.append b d) (S.length b + (S.length d / l) * l) (S.length (S.append b d));
+  (S.equal) { Math.Lemmas.div_exact_r (S.length b) l }
+    // For some reason this doesn't go through with the default rlimit, even
+    // though this is a direct rewriting based on the application of the lemma
+    // above.
+    S.slice (S.append b d) ((S.length b / l) * l + (S.length d / l) * l) (S.length (S.append b d));
+  (S.equal) { Math.Lemmas.distributivity_add_left (S.length b / l) (S.length d / l) l }
+    S.slice (S.append b d) ((S.length b / l + S.length d / l) * l) (S.length (S.append b d));
+  (S.equal) { Math.Lemmas.lemma_div_plus (S.length d) (S.length b / l) l }
+    S.slice (S.append b d) (((S.length b + S.length d) / l) * l) (S.length (S.append b d));
+  (S.equal) { }
+    snd (S.split (S.append b d) (((S.length (S.append b d)) / l) * l));
+  (S.equal) { }
+    rest'';
+  };
+
+  calc (S.equal) {
+    S.append blocks blocks';
+  (S.equal) { (* rest = S.empty *) }
+    S.append (S.append blocks rest) blocks';
+  (S.equal) { }
+    S.append b blocks';
+  (S.equal) { }
+    S.append b (fst (split_at_last c i d));
+  (S.equal) { (* definition of split_at_last *) }
+    S.append b (fst (S.split d ((S.length d / l) * l)));
+  (S.equal) { (* definition of split *) }
+    S.append b (S.slice d 0 ((S.length d / l) * l));
+  (S.equal) { }
+    S.slice (S.append b d) 0 (S.length b + (S.length d / l) * l);
+  (S.equal) { Math.Lemmas.div_exact_r (S.length b) l }
+    S.slice (S.append b d) 0 ((S.length b / l) * l + (S.length d / l) * l);
+  (S.equal) { Math.Lemmas.distributivity_add_left (S.length b / l) (S.length d / l) l }
+    S.slice (S.append b d) 0 ((S.length b / l + S.length d / l) * l);
+  (S.equal) { Math.Lemmas.lemma_div_plus (S.length d) (S.length b / l) l }
+    S.slice (S.append b d) 0 (((S.length b + S.length d) / l) * l);
+  (S.equal) { }
+    fst (S.split (S.append b d) (((S.length (S.append b d)) / l) * l));
+  (S.equal) { }
+    blocks'';
+  }
+
+#push-options "--z3rlimit 50"
+val update_empty_buf:
+  #index:Type0 ->
+  c:block index ->
+  i:G.erased index -> (
+  let i = G.reveal i in
+  s:state c i ->
+  data: B.buffer Lib.IntTypes.uint8 ->
+  len: UInt32.t ->
+  Stack unit
+    (requires fun h0 ->
+      update_pre c i s data len h0 /\
+      rest c i (total_len_h c i h0 s) = 0ul)
+    (ensures fun h0 s' h1 ->
+      update_post c i s data len h0 h1))
+
+inline_for_extraction noextract
+let seen_pred = seen
+
+let update_empty_buf #index c i p data len =
+  let aux (h:HS.mem) (s:c.state i): Lemma
+    (requires (c.invariant h s))
+    (ensures (B.loc_in (c.footprint #i h s) h))
+    [SMTPat (c.invariant h s)]
+  =
+    c.invariant_loc_in_footprint #i h s
+  in
+  let aux l s h0 h1: Lemma
+    (requires
+      c.invariant h0 s /\
+      c.freeable h0 s /\
+      B.loc_disjoint l (c.footprint #i h0 s) /\
+      B.modifies l h0 h1)
+    (ensures (
+      c.freeable h1 s))
+    [ SMTPat (c.freeable h1 s); SMTPat (B.modifies l h0 h1) ]
+  =
+    c.frame_freeable #i l s h0 h1
+  in
+  let aux i h
+    (input1:S.seq uint8 { S.length input1 % U32.v (c.block_len i) = 0 })
+    (input2:S.seq uint8 { S.length input2 % U32.v (c.block_len i) = 0 }):
+    Lemma (ensures (
+      let input = S.append input1 input2 in
+      concat_blocks_modulo (U32.v (c.block_len i)) input1 input2;
+      (==) (c.update_multi_s i (c.update_multi_s i h input1) input2)
+        (c.update_multi_s i h input)))
+    [ SMTPat (c.update_multi_s i (c.update_multi_s i h input1) input2) ]
+  =
+    c.update_multi_associative i h input1 input2
+  in
+  
+  let open LowStar.BufferOps in
+  let s = !*p in
+  let State hash_state buf total_len seen = s in
+  let i = c.index_of_state i hash_state in
+  [@inline_let]
+  let hash_state: c.state i = hash_state in
+  let sz = rest c i total_len in
+  let h0 = ST.get () in
+  assert (
+    let blocks, rest = split_at_last c i (G.reveal seen) in
+    S.equal blocks (G.reveal seen) /\
+    S.equal rest S.empty);
+  split_at_last_blocks c i (G.reveal seen) (B.as_seq h0 data);
+  let n_blocks = len `U32.div` c.block_len i in
+  let data1_len = n_blocks `U32.mul` c.block_len i in
+  let data2_len = len `U32.sub` data1_len in
+  let data1 = B.sub data 0ul data1_len in
+  let data2 = B.sub data data1_len data2_len in
+  c.update_multi (G.hide i) hash_state data1 data1_len;
+
+  let dst = B.sub buf 0ul data2_len in
+  let h1 = ST.get () in
+  B.blit data2 0ul dst 0ul data2_len;
+  let h2 = ST.get () in
+  c.frame_invariant (B.loc_buffer buf) hash_state h1 h2;
+
+  S.append_assoc (G.reveal seen) (B.as_seq h0 data1) (B.as_seq h0 data2);
+  assert (S.equal
+    (S.append (S.append (G.reveal seen) (B.as_seq h0 data1)) (B.as_seq h0 data2))
+    (S.append (G.reveal seen) (S.append (B.as_seq h0 data1) (B.as_seq h0 data2))));
+
+  p *= (State hash_state buf (add_len c i total_len len)
+    (G.hide (G.reveal seen `S.append` B.as_seq h0 data)));
+  let h3 = ST.get () in
+  c.frame_invariant (B.loc_buffer p) hash_state h2 h3;
+
+  // After careful diagnosis, this is the difficult proof obligation that sends
+  // z3 off the rails.
+  (
+    let seen' = G.reveal seen `S.append` B.as_seq h0 data in
+    let blocks, rest = split_at_last c i seen' in
+    calc (==) {
+      S.length blocks + S.length rest;
+    (==) { }
+      S.length seen';
+    (==) { S.lemma_len_append (G.reveal seen) (B.as_seq h0 data) }
+      S.length (G.reveal seen) + S.length (B.as_seq h0 data);
+    (==) { }
+      U64.v total_len + U32.v len;
+    }
+  )
+#pop-options
+
+
+/// Case 3: we are given just enough data to end up on the boundary
+#push-options "--z3rlimit 200"
+val update_round:
+  #index:Type0 ->
+  c:block index ->
+  i:G.erased index -> (
+  let i = G.reveal i in
+  s:state c i ->
+  data: B.buffer uint8 ->
+  len: UInt32.t ->
+  Stack unit
+    (requires fun h0 ->
+      update_pre c i s data len h0 /\ (
+      let r = rest c i (total_len_h c i h0 s) in
+      U32.v len + U32.v r = U32.v (c.block_len i) /\
+      r <> 0ul))
+    (ensures fun h0 _ h1 ->
+      update_post c i s data len h0 h1 /\
+      U64.v (total_len_h c i h1 s) % U32.v (c.block_len i) = 0))
+
+(*let split_at_last_block #index (c: block index) (i: index) (b: bytes) (d: bytes): Lemma
+  (requires (
+    let _, rest = split_at_last c i b in
+    S.length rest + S.length d = U32.v (c.block_len i)))
+  (ensures (
+    let blocks, rest = split_at_last c i b in
+    let blocks', rest' = split_at_last c i (S.append b d) in
+    S.equal (S.append b d) blocks' /\ S.equal S.empty rest'))
+=
+   admit ()
+
+let update_round #index c i p data len =
+  let aux (h:HS.mem) (s:c.state i): Lemma
+    (requires (c.invariant h s))
+    (ensures (B.loc_in (c.footprint #i h s) h))
+    [SMTPat (c.invariant h s)]
+  =
+    c.invariant_loc_in_footprint #i h s
+  in
+  let aux l s h0 h1: Lemma
+    (requires
+      c.invariant h0 s /\
+      c.freeable h0 s /\
+      B.loc_disjoint l (c.footprint #i h0 s) /\
+      B.modifies l h0 h1)
+    (ensures (
+      c.freeable h1 s))
+    [ SMTPat (c.freeable h1 s); SMTPat (B.modifies l h0 h1) ]
+  =
+    c.frame_freeable #i l s h0 h1
+  in
+  let aux i h
+    (input1:S.seq uint8 { S.length input1 % U32.v (c.block_len i) = 0 })
+    (input2:S.seq uint8 { S.length input2 % U32.v (c.block_len i) = 0 }):
+    Lemma (ensures (
+      let input = S.append input1 input2 in
+      concat_blocks_modulo (U32.v (c.block_len i)) input1 input2;
+      (==) (c.update_multi_s i (c.update_multi_s i h input1) input2)
+        (c.update_multi_s i h input)))
+    [ SMTPat (c.update_multi_s i (c.update_multi_s i h input1) input2) ]
+  =
+    c.update_multi_associative i h input1 input2
+  in
+
+  let open LowStar.BufferOps in
+  let s = !*p in
+  let State hash_state buf_ total_len seen = s in
+  let i = c.index_of_state i hash_state in
+  [@inline_let]
+  let hash_state: c.state i = hash_state in
+  let h0 = ST.get () in
+  let sz = rest c i total_len in
+  let diff = c.block_len i `U32.sub` sz in
+  let buf0 = B.sub buf_ 0ul (c.block_len i) in
+  let buf1 = B.sub buf0 0ul sz in
+  let buf2 = B.sub buf0 sz diff in
+  assert (B.(loc_pairwise_disjoint
+    [ loc_buffer buf1; loc_buffer buf2; loc_buffer data; ]));
+  B.blit data 0ul buf2 0ul diff;
+  let h1 = ST.get () in
+  assert (S.equal (B.as_seq h1 buf0) (S.append (B.as_seq h1 buf1) (B.as_seq h1 data)));
+  c.frame_invariant (B.loc_buffer buf_) hash_state h0 h1;
+  c.update_multi (G.hide i) hash_state buf0 (c.block_len i);
+  let h2 = ST.get () in
+  // JP: no clue why I had to go through all these manual steps.
+  (
+    let blocks, rest = split_at_last c i (G.reveal seen) in
+    assert ((==) (c.v h2 hash_state)
+      (c.update_multi_s i (c.v h1 hash_state) (B.as_seq h1 buf0)));
+    assert (S.equal (B.as_seq h0 buf1) (B.as_seq h1 buf1));
+    assert (S.equal rest (B.as_seq h1 buf1));
+    assert (S.equal (B.as_seq h0 data) (B.as_seq h1 data));
+    assert (S.equal (B.as_seq h1 buf0) (S.append (B.as_seq h1 buf1) (B.as_seq h1 data)));
+    assert ((==) (c.v h2 hash_state)
+      (c.update_multi_s i (c.init_s i)
+        (S.append blocks (B.as_seq h1 buf0))));
+    assert ((==) (c.v h2 hash_state)
+      (c.update_multi_s i (c.init_s i)
+        (S.append blocks (S.append (B.as_seq h1 buf1) (B.as_seq h1 data)))));
+    ()); admit ()
+    S.append_assoc blocks (B.as_seq h1 buf1) (B.as_seq h1 data);
+    assert (S.equal (c.v h2 hash_state)
+      (update_multi i (Spec.Agile.Hash.init i)
+        (S.append (S.append blocks (B.as_seq h1 buf1)) (B.as_seq h1 data))));
+    assert (S.equal (S.append blocks rest) (G.reveal seen));
+    assert (S.equal (c.v h2 hash_state)
+      (update_multi i (Spec.Agile.Hash.init i)
+        (S.append (G.reveal seen) (B.as_seq h1 data))));
+    assert (S.equal (c.v h2 hash_state)
+      (update_multi i (Spec.Agile.Hash.init i)
+        (S.append (G.reveal seen) (B.as_seq h0 data))));
+    split_at_last_block i (G.reveal seen) (B.as_seq h0 data);
+    let blocks', rest' = split_at_last i (S.append (G.reveal seen) (B.as_seq h0 data)) in
+    assert (S.equal rest' S.empty);
+    assert (B.live h2 buf_ /\
+      B.(loc_disjoint (loc_buffer buf_) (Hash.footprint hash_state h2)) /\
+      Hash.invariant hash_state h2);
+    ()
+  );
+  p *= (State hash_state buf_ (add_len total_len len)
+    (G.hide (G.reveal seen `S.append` B.as_seq h0 data)));
+  let h3 = ST.get () in
+  Hash.frame_invariant (B.loc_buffer p) hash_state h2 h3;
+  Hash.frame_invariant_implies_footprint_preservation (B.loc_buffer p) hash_state h2 h3;
+  assert (hashed #i h3 p `S.equal` (S.append (G.reveal seen) (B.as_seq h0 data)))
+#pop-options
+
+#push-options "--z3rlimit 200"
+let update a p data len =
+  let open LowStar.BufferOps in
+  let s = !*p in
+  let State hash_state buf_ total_len seen = s in
+  let a = Hash.alg_of_state a hash_state in
+  let sz = rest a total_len in
+  if len `U32.lt` (Hacl.Hash.Definitions.block_len a `U32.sub` sz) then
+    update_small (G.hide a) p data len
+  else if sz = 0ul then
+    update_empty_buf (G.hide a) p data len
+  else begin
+    let h0 = ST.get () in
+    let diff = Hacl.Hash.Definitions.block_len a `U32.sub` sz in
+    let data1 = B.sub data 0ul diff in
+    let data2 = B.sub data diff (len `U32.sub` diff) in
+    update_round (G.hide a) p data1 diff;
+    let h1 = ST.get () in
+    update_empty_buf (G.hide a) p data2 (len `U32.sub` diff);
+    let h2 = ST.get () in
+    (
+      let seen = G.reveal seen in
+      assert (hashed #a h1 p `S.equal` (S.append seen (B.as_seq h0 data1)));
+      assert (hashed #a h2 p `S.equal` (S.append (S.append seen (B.as_seq h0 data1)) (B.as_seq h0 data2)));
+      S.append_assoc seen (B.as_seq h0 data1) (B.as_seq h0 data2);
+      assert (S.equal (S.append (B.as_seq h0 data1) (B.as_seq h0 data2)) (B.as_seq h0 data));
+      assert (S.equal
+        (S.append (S.append seen (B.as_seq h0 data1)) (B.as_seq h0 data2))
+        (S.append seen (B.as_seq h0 data)));
+      assert (hashed #a h2 p `S.equal` (S.append seen (B.as_seq h0 data)));
+      ()
+    )
+  end
+#pop-options
+
+*)
